specs/ecdsap256sha2/Spec.P256.MontgomeryMultiplication.fsti
@@ -8,6 +8,7 @@ open Spec.P256.Lemmas
 open Spec.P256.Definitions
 
 open Lib.IntTypes
+open Lib.Sequence
 
 #set-options "--z3rlimit 40 --fuel 0 --ifuel 0"
 
@@ -52,3 +53,28 @@ val additionInDomain: a: nat {a < prime256} -> b: nat {b < prime256} -> Lemma
   
 val substractionInDomain: a: nat {a < prime256} -> b: nat { b < prime256} -> Lemma 
   ((a - b) % prime256 == toDomain_ (fromDomain_ a - fromDomain_ b))
+
+
+val _pow_step0: p:nat_prime -> q:nat_prime -> tuple2 nat_prime nat_prime
+
+val _pow_step1: p:nat_prime -> q:nat_prime -> tuple2 nat_prime nat_prime
+
+let swap (p:nat_prime) (q:nat_prime) = q, p
+
+val conditional_swap_pow: i:uint64 -> p:nat_prime -> q:nat_prime -> tuple2 nat_prime nat_prime
+
+val lemma_swaped_steps: p: nat_prime -> q: nat_prime ->
+  Lemma (
+    let afterSwapP, afterSwapQ = swap p q in
+    let p1, q1 = _pow_step0 afterSwapP afterSwapQ in
+    let p2, q2 = swap p1 q1 in
+    let r0, r1 = _pow_step1 p q in
+    p2 == r0 /\ q2 == r1)
+
+
+val _pow_step: k:lseq uint8 32 -> i:nat{i < 256} -> before:tuple2 nat_prime nat_prime
+  -> tuple2 nat_prime nat_prime
+
+
+val pow_spec: k:lseq uint8 32  -> tuple2 nat_prime nat_prime
+  -> tuple2 nat_prime nat_prime
