specs/ecdsap256sha2/Spec.P256.fst
@@ -16,9 +16,6 @@ open FStar.Math.Lib
 
 let prime = prime256
 
-let nat_prime = n:nat{n < prime}
-
-
 let aCoordinateP256 = -3 
 let bCoordinateP256 : (a: nat {a < prime256}) =
   assert_norm (41058363725152142129326129780047268409114441015993725554835256314039467401291 < prime256);
@@ -212,60 +209,3 @@ let point_prime_to_coordinates (p:point_seq) =
 val toJacobianCoordinates: tuple2 nat nat -> tuple3 nat nat nat
 let toJacobianCoordinates (r0, r1) = (r0, r1, 1)
 
-
-
-let ( *% ) a b = (a * b) % prime
-
-
-val _exp_step0: p:nat_prime -> q:nat_prime -> tuple2 nat_prime nat_prime
-
-let _exp_step0 r0 r1 =
-  let r1 = r0 *% r1 in
-  let r0 = r0 *% r0 in
-  r0, r1
-
-
-val _exp_step1: p:nat_prime -> q:nat_prime -> tuple2 nat_prime nat_prime
-
-let _exp_step1 r0 r1 =
-  let r0 = r0 *% r1 in
-  let r1 = r1 *% r1 in
-  (r0, r1)
-
-
-let swap (p:nat_prime) (q:nat_prime) = q, p
-
-
-val conditional_swap_exponent: i:uint64 -> p:nat_prime -> q:nat_prime -> tuple2 nat_prime nat_prime
-
-let conditional_swap_exponent i p q =
-  if v i = 0 then (p, q) else (q, p)
-
-
-val lemma_swaped_steps: p: nat_prime -> q: nat_prime ->
-  Lemma (
-    let afterSwapP, afterSwapQ = swap p q in
-    let p1, q1 = _exp_step0 afterSwapP afterSwapQ in
-    let p2, q2 = swap p1 q1 in
-    let r0, r1 = _exp_step1 p q in
-    p2 == r0 /\ q2 == r1)
-
-let lemma_swaped_steps p q = ()
-
-
-val _exp_step: k:lseq uint8 32 -> i:nat{i < 256} -> before:tuple2 nat_prime nat_prime
-  -> tuple2 nat_prime nat_prime
-
-let _exp_step k i (p, q) =
-  let bit = 255 - i in
-  let bit = ith_bit k bit in
-  let open Lib.RawIntTypes in
-  if uint_to_nat bit = 0 then _exp_step0 p q else _exp_step1 p q
-
-
-val _exponent_spec: k:lseq uint8 32  -> tuple2 nat_prime nat_prime
-  -> tuple2 nat_prime nat_prime
-
-let _exponent_spec k (p, q) =
-  let open Lib.LoopCombinators in
-  Lib.LoopCombinators.repeati 256 (_exp_step k) (p, q)
