code/ecdsap256sha2/Hacl.Impl.P256.MM.Exponent.fsti
@@ -1,0 +1,36 @@
+module Hacl.Impl.P256.MM.Exponent
+
+open FStar.HyperStack.All
+open FStar.HyperStack
+module ST = FStar.HyperStack.ST
+
+open Lib.IntTypes
+open Lib.Buffer
+
+open FStar.Math.Lemmas
+open Hacl.Impl.P256.Math 
+
+open Hacl.Impl.LowLevel
+open FStar.Tactics
+open FStar.Tactics.Canon 
+
+open FStar.Mul
+
+open Lib.Loops
+
+open Hacl.Impl.P256.MontgomeryMultiplication
+open Spec.P256.MontgomeryMultiplication
+
+open Hacl.Impl.P256.LowLevel
+open Hacl.Impl.P256
+open Hacl.Impl.P256.Arithmetics
+
+open Spec.P256.Definitions
+open Spec.P256.Lemmas
+open Spec.P256
+open Spec.P256.Ladder
+open Spec.P256.MontgomeryMultiplication
+
+val square_root: a: felem -> Stack unit 
+  (requires fun h -> True)
+  (ensures fun h0 _ h1 -> True)
